Refactor: use def for proof systems and move form's out of Semantics and ProofSystem structures

Modal/common/logic.lean
@@ -1,53 +1,54 @@
-/- I use `Type _` to allow those types to live in any
-universe at any level. If I omit that and, for example,
-the field `Semantics.model` is defined in some instance
-depending on another type, like `Atom`, there would be
-universe inconsistencies. -/
+/- I need `Type _` (with the underscore) to allow those types to live in any
+universe at any level. If I omit that and, for example, the field
+`Semantics.model` is defined in some instance depending on another type,
+like `Atom`, there would be universe inconsistencies. -/
 
 
 import Mathlib.Data.Set.Defs
 
-
 namespace Logic
 
-class ProofSystem where
-  form : Type _  -- formulas
-  entails : Set form → form → Prop
-notation:50 Γ " ⊢[" P "] " φ => (fun Γ P φ => P.entails Γ φ)
+structure ProofSystem (Form : Type _) where
+  entails : Set Form → Form → Prop
+notation:50 Γ " ⊢[" ps "] " φ => ProofSystem.entails ps Γ φ
 
-def is_tauto (P : ProofSystem) (φ : P.form) : Prop :=
-  P.entails ∅ φ
-notation:50 "⊢[" P "] " φ => (fun P φ => P.is_tauto φ)
+namespace ProofSystem
 
+def is_tauto {Form : Type _} (ps : ProofSystem Form) (φ : Form) : Prop :=
+  ps.entails ∅ φ
+notation:50 "⊢[" ps "] " φ => is_tauto ps φ
 
-class Semantics where
-  form : Type _  -- formulas
-  model : Type _  -- models
-  satisfies : model → form → Prop
-
-def is_sem_conseq (S : Semantics) (Γ : Set S.form) (φ : S.form) : Prop :=
-  ∀ (M : S.model), (∀ ψ ∈ Γ, S.satisfies M ψ) → S.satisfies M φ
-notation:50 Γ " ⊨[" S "] " φ:50 => is_sem_conseq S Γ φ
-
-def is_valid (S : Semantics) (φ : S.form) : Prop :=
-  is_sem_conseq S ∅ φ
-notation:50 "⊨[" S "] " φ => (fun S φ => S.is_valid φ)
+end ProofSystem
 
 
--- We need to tell Lean how to convert ps.form into sem.form,
--- that's why Γ' and φ'.
-def is_sound (ps : ProofSystem) (sem : Semantics)
-             (h_eq_form : ps.form = sem.form) : Prop :=
-  ∀ (Γ : Set ps.form) (φ : ps.form),
-    let Γ' := Set.image (Eq.mp h_eq_form) Γ
-    let φ' := Eq.mp h_eq_form φ
-    ps.entails Γ φ → is_sem_conseq sem Γ' φ'
+structure Semantics (Form : Type _) where
+  model : Type _
+  satisfies : model → Form → Prop
 
-def is_complete (ps : ProofSystem) (sem : Semantics)
-                (h_eq_form : ps.form = sem.form) : Prop :=
-  ∀ (Γ : Set ps.form) (φ : ps.form),
-    let Γ' := Set.image (Eq.mp h_eq_form) Γ
-    let φ' := Eq.mp h_eq_form φ
-    is_sem_conseq sem Γ' φ' → ps.entails Γ φ
+namespace Semantics
+
+def is_sem_conseq {Form : Type _} (sem : Semantics Form)
+    (Γ : Set Form) (φ : Form) : Prop :=
+  ∀ (M : sem.model), (∀ ψ ∈ Γ, sem.satisfies M ψ) → sem.satisfies M φ
+notation:50 Γ " ⊨[" sem "] " φ => is_sem_conseq sem Γ φ
+
+def is_valid {Form : Type _} (sem : Semantics Form) (φ : Form) : Prop :=
+  sem.is_sem_conseq ∅ φ
+notation:50 "⊨[" sem "] " φ => is_valid sem φ
+
+end Semantics
+
+
+def is_sound_strong {Form : Type _} (ps : ProofSystem Form) (sem : Semantics Form) : Prop :=
+  ∀ (Γ : Set Form) (φ : Form), (Γ ⊢[ps] φ) → (Γ ⊨[sem] φ)
+
+def is_sound_weak {Form : Type _} (ps : ProofSystem Form) (sem : Semantics Form) : Prop :=
+  ∀ (φ : Form), (⊢[ps] φ) → (⊨[sem] φ)
+
+def is_complete_strong {Form : Type _} (ps : ProofSystem Form) (sem : Semantics Form) : Prop :=
+  ∀ (Γ : Set Form) (φ : Form), (Γ ⊨[sem] φ) → (Γ ⊢[ps] φ)
+
+def is_complete_weak {Form : Type _} (ps : ProofSystem Form) (sem : Semantics Form) : Prop :=
+  ∀ (φ : Form), (⊨[sem] φ) → (⊢[ps] φ)
 
 end Logic
