Modal/cpl/proof.lean
@@ -5,9 +5,8 @@ import Modal.cpl.formula
 
 namespace CPL
 
-def proof_system (Atom : Type) : Logic.ProofSystem :=
-  { form := Formula Atom
-    entails : Set (Formula Atom) → Formula Atom → Prop := by admit }
+def proof_system (Atom : Type) : Logic.ProofSystem (Formula Atom) :=
+  { entails := fun _ _ => by admit }
 
 
 structure Valuation (Form : Type) [Syntax Form] where
@@ -15,18 +14,17 @@ structure Valuation (Form : Type) [Syntax Form] where
   h_val_bot : val ⊥ = False
   h_val_impl : ∀ φ ψ, val (φ → ψ) = (val φ → val ψ)
 
-def semantics (Atom : Type) : Logic.Semantics :=
-  { form := Formula Atom
-    model := Valuation (Formula Atom)
+def semantics (Atom : Type) : Logic.Semantics (Formula Atom) :=
+  { model := Valuation (Formula Atom)
     satisfies := fun v φ => v.val φ }
 
 
-theorem is_sound (Atom : Type) :
-    Logic.is_sound (proof_system Atom) (semantics Atom) (by rfl) :=
+theorem is_sound_strong (Atom : Type) :
+    Logic.is_sound_strong (proof_system Atom) (semantics Atom) :=
   by admit
 
-theorem is_complete (Atom : Type) :
-     Logic.is_complete (proof_system Atom) (semantics Atom) (by rfl) :=
+theorem is_complete_strong (Atom : Type) :
+     Logic.is_complete_strong (proof_system Atom) (semantics Atom) :=
   by admit
 
 /- TODO: I may need to define specific proof systems and semantics for CPL.
