Modal/modal/sound_complete/K_kripke.lean
@@ -9,12 +9,13 @@ open Modal.ProofSystems Modal.Models
 
 def all_frames : Kripke.Frame → Prop := fun _ => True
 
-theorem is_sound (Atom : Type) :
-    Logic.is_sound (K.proof_system Atom) (@Kripke.semantics Atom all_frames) (by rfl) :=
+theorem is_sound_strong (Atom : Type) :
+    Logic.is_sound_strong (K.proof_system Atom) (@Kripke.semantics Atom all_frames) :=
   by admit
 
-theorem is_complete (Atom : Type) :
-     Logic.is_complete (K.proof_system Atom) (@Kripke.semantics Atom all_frames) (by rfl) :=
+theorem is_complete_weak (Atom : Type) :
+     Logic.is_complete_weak (K.proof_system Atom) (@Kripke.semantics Atom all_frames) :=
   by admit
+-- K is not strongly complete wrt Kripke models
 
 end Modal.SoundComplete.K_Kripke
