Modal/modal/sound_complete/M_upnbhd.lean
@@ -10,12 +10,13 @@ open Modal.ProofSystems Modal.Models
 def is_upclosed : Nbhd.Frame → Prop :=
   fun f => ∀ w (X Y : Set f.world), X ∈ f.nbhd w → X ⊆ Y → Y ∈ f.nbhd w
 
-theorem is_sound (Atom : Type) :
-    Logic.is_sound (E.proof_system Atom) (@Nbhd.semantics Atom is_upclosed) (by rfl) :=
+theorem is_sound_strong (Atom : Type) :
+    Logic.is_sound_strong (E.proof_system Atom) (@Nbhd.semantics Atom is_upclosed) :=
   by admit
 
-theorem is_complete (Atom : Type) :
-    Logic.is_complete (E.proof_system Atom) (@Nbhd.semantics Atom is_upclosed) (by rfl) :=
+theorem is_complete_weak (Atom : Type) :
+    Logic.is_complete_weak (E.proof_system Atom) (@Nbhd.semantics Atom is_upclosed) :=
   by admit
+-- M is not strongly complete wrt upclosed neighbourhood models
 
 end Modal.SoundComplete.M_UpNbhd
